otbn_model/code/mont_loop_lemmas.dfy
@@ -308,4 +308,7 @@ module mont_loop_lemmas {
                 x_i * to_nat(y) + u_i * to_nat(m) + to_nat(initial_a), to_nat(m));
         }
     }
+
+
+    predicate montmul_inv()
 }
